code/poly1305/Hacl.Impl.Poly1305.fsti
@@ -15,8 +15,8 @@ module F32xN = Hacl.Impl.Poly1305.Field32xN
 
 #reset-options "--z3rlimit 50"
 
-inline_for_extraction
-type poly1305_ctx (s:field_spec) = lbuffer (limb s) (nlimb s +. precomplen s)
+inline_for_extraction noextract
+let poly1305_ctx (s:field_spec) = lbuffer (limb s) (nlimb s +. precomplen s)
 
 noextract
 val as_get_acc: #s:field_spec -> h:mem -> ctx:poly1305_ctx s -> GTot (S.elem (width s))
@@ -25,7 +25,17 @@ val as_get_r: #s:field_spec -> h:mem -> ctx:poly1305_ctx s -> GTot (S.elem (widt
 noextract
 val state_inv_t: #s:field_spec -> h:mem -> ctx:poly1305_ctx s -> Type0
 
-inline_for_extraction
+// If the ctx is not modified, all the components and invariants are preserved
+val reveal_ctx_inv: #s:field_spec -> ctx:poly1305_ctx s -> h0:mem -> h1:mem ->
+  Lemma
+    (requires Seq.equal (as_seq h0 ctx) (as_seq h1 ctx) /\ state_inv_t h0 ctx)
+    (ensures 
+      as_get_r h0 ctx == as_get_r h1 ctx /\
+      as_get_acc h0 ctx == as_get_acc h1 ctx /\
+      state_inv_t h1 ctx
+    )
+
+inline_for_extraction noextract
 val poly1305_init:
     #s:field_spec
   -> ctx:poly1305_ctx s
@@ -38,7 +48,7 @@ val poly1305_init:
       state_inv_t #s h1 ctx /\
       (as_get_acc h1 ctx, as_get_r h1 ctx) == S.poly1305_init (as_seq h0 key))
 
-inline_for_extraction
+inline_for_extraction noextract
 val poly1305_update:
     #s:field_spec
   -> ctx:poly1305_ctx s
@@ -51,10 +61,11 @@ val poly1305_update:
     (ensures  fun h0 _ h1 ->
       modifies (loc ctx) h0 h1 /\
       state_inv_t #s h1 ctx /\
+      as_get_r h0 ctx == as_get_r h1 ctx /\
       Lib.Sequence.index (as_get_acc h1 ctx) 0 ==
       S.poly_update #(width s) (as_seq h0 text) (as_get_acc h0 ctx) (as_get_r h0 ctx))
 
-inline_for_extraction
+inline_for_extraction noextract
 val poly1305_finish:
     #s:field_spec
   -> tag:lbuffer uint8 16ul
@@ -69,7 +80,7 @@ val poly1305_finish:
       modifies (loc tag |+| loc ctx) h0 h1 /\
       as_seq h1 tag == S.finish (as_seq h0 key) (Lib.Sequence.index (as_get_acc h0 ctx) 0))
 
-inline_for_extraction
+inline_for_extraction noextract
 val poly1305_mac:
     #s:field_spec
   -> tag:lbuffer uint8 16ul
