code/experimental/chacha20/Hacl.Impl.Chacha20.Core32.fst
@@ -15,13 +15,13 @@ let index = (i:size_t{size_v i < 16})
 inline_for_extraction
 val create_state: unit -> StackInline state
 		  (requires (fun h -> True))
-   		  (ensures (fun h0 r h1 -> live h1 r /\ 
+   		  (ensures (fun h0 r h1 -> live h1 r /\
 					as_seq h1 r == Seq.create 16 (u32 0) /\
 					stack_allocated r h0 h1 (Seq.create 16 (u32 0))))
-let create_state () = create (size 16) (u32 0) 
+let create_state () = create (size 16) (u32 0)
 
 inline_for_extraction
-val load_state: st:state -> b:lbuffer uint8 64ul -> ST unit
+val load_state: st:state -> b:lbuffer uint8 64ul -> Stack unit
 		  (requires (fun h -> live h st /\ live h b /\ disjoint st b))
    		  (ensures (fun h0 _ h1 -> modifies (loc st) h0 h1 /\
 			   as_seq h1 st == Lib.ByteSequence.uints_from_bytes_le (as_seq h0 b)))
@@ -29,7 +29,7 @@ let load_state st b =
     uints_from_bytes_le st b
 
 inline_for_extraction
-val store_state: b:lbuffer uint8 64ul -> st:state -> ST unit
+val store_state: b:lbuffer uint8 64ul -> st:state -> Stack unit
 		  (requires (fun h -> live h st /\ live h b /\ disjoint st b))
    		  (ensures (fun h0 _ h1 -> modifies (loc b) h0 h1 /\
 		    as_seq h1 b == Lib.ByteSequence.uints_to_bytes_le (as_seq h0 st)))
@@ -37,7 +37,7 @@ let store_state st b =
     uints_to_bytes_le 16ul st b
 
 inline_for_extraction
-val set_counter: st:state -> c:size_t -> ST unit
+val set_counter: st:state -> c:size_t -> Stack unit
 		  (requires (fun h -> live h st))
    		  (ensures (fun h0 _ h1 -> modifies (loc st) h0 h1 /\
 			   as_seq h1 st == Seq.upd (as_seq h0 st) 12 (size_to_uint32 c)))
@@ -45,7 +45,7 @@ let set_counter st c =
     st.(size 12) <- size_to_uint32 c
 
 inline_for_extraction
-val incr_counter: st:state -> ST unit
+val incr_counter: st:state -> Stack unit
 		  (requires (fun h -> live h st))
    		  (ensures (fun h0 _ h1 -> modifies (loc st) h0 h1))
 let incr_counter st =
@@ -53,25 +53,25 @@ let incr_counter st =
     st.(size 12) <- c +. u32 1
 
 inline_for_extraction
-val copy_state: st:state -> ost:state -> ST unit
+val copy_state: st:state -> ost:state -> Stack unit
 		  (requires (fun h -> live h st /\ live h ost /\ disjoint st ost))
-   		  (ensures (fun h0 _ h1 -> 
+   		  (ensures (fun h0 _ h1 ->
 		    modifies (loc st) h0 h1 /\
 		    as_seq h1 st == as_seq h0 ost))
 let copy_state st ost = copy #MUT #uint32 #(size 16) st ost
 
 
 inline_for_extraction
-val sum_state: st:state -> ost:state -> ST unit
+val sum_state: st:state -> ost:state -> Stack unit
 		  (requires (fun h -> live h st /\ live h ost /\ eq_or_disjoint st ost))
-   		  (ensures (fun h0 _ h1 -> 
-		    modifies (loc st) h0 h1 /\ 
+   		  (ensures (fun h0 _ h1 ->
+		    modifies (loc st) h0 h1 /\
 		    as_seq h1 st == Spec.sum_state (as_seq h0 st) (as_seq h0 ost)))
 let sum_state st ost =  map2T #MUT #uint32 #uint32 #uint32 (size 16) st ( +. ) st ost
-      
+
 
 inline_for_extraction
-val xor_block: o:lbuffer uint8 64ul -> st:state -> b:lbuffer uint8 64ul -> ST unit
+val xor_block: o:lbuffer uint8 64ul -> st:state -> b:lbuffer uint8 64ul -> Stack unit
 		  (requires (fun h -> live h o /\ live h st /\ live h b))
    		  (ensures (fun h0 _ h1 -> modifies (loc o) h0 h1 /\
 					as_seq h1 o == Spec.xor_block (as_seq h0 st) (as_seq h0 b)))
@@ -83,15 +83,15 @@ let xor_block o st b =
     map2T (size 16) bl ( ^. ) bl st;
     store_state o bl;
     pop_frame()
-    
+
 
 
 inline_for_extraction
-val line: st:state -> a:index -> b:index -> d:index -> r:rotval U32 -> ST unit
+val line: st:state -> a:index -> b:index -> d:index -> r:rotval U32 -> Stack unit
 		  (requires (fun h -> live h st /\ v a <> v d))
 		  (ensures (fun h0 _ h1 -> modifies (loc st) h0 h1 /\
 		    as_seq h1 st == Spec.line (v a) (v b) (v d) r (as_seq h0 st)))
-let line st a b d r = 
+let line st a b d r =
   let sta = st.(a) in
   let stb = st.(b) in
   let std = st.(d) in
@@ -102,24 +102,24 @@ let line st a b d r =
   st.(d) <- std
 
 inline_for_extraction
-val quarter_round: st:state -> a:index -> b:index -> c:index -> d:index -> ST unit
+val quarter_round: st:state -> a:index -> b:index -> c:index -> d:index -> Stack unit
 		  (requires (fun h -> live h st /\ v a <> v d /\ v c <> v b))
 		  (ensures (fun h0 _ h1 -> modifies (loc st) h0 h1 /\
 			   as_seq h1 st == Spec.quarter_round (v a) (v b) (v c) (v d) (as_seq h0 st)))
 [@ CInline ]
-let quarter_round st a b c d = 
+let quarter_round st a b c d =
     line st a b d (size 16);
     line st c d b (size 12);
     line st a b d (size 8);
     line st c d b (size 7)
 
 [@ CInline]
-val double_round: st:state -> ST unit
+val double_round: st:state -> Stack unit
 		  (requires (fun h -> live h st))
 		  (ensures (fun h0 _ h1 -> modifies (loc st) h0 h1 /\
 		    as_seq h1 st == Spec.double_round (as_seq h0 st)))
 [@ CInline]
-let double_round st = 
+let double_round st =
   quarter_round st (size 0) (size 4) (size 8) (size 12);
   quarter_round st (size 1) (size 5) (size 9) (size 13);
   quarter_round st (size 2) (size 6) (size 10) (size 14);
