code/poly1305/Hacl.Spec.Poly1305.Field32xN.fst
@@ -52,12 +52,15 @@ let ( <=* ) (x:nat5) (y:nat5) : Type =
   (x4 <= y4) /\
   (x5 <= y5)
 
-assume val pow26: nat
+abstract
+let pow26: (pow26: pos { pow2 32 == 64 * pow26 /\ pow2 64 == 4096 * pow26 * pow26 /\ pow26 == pow2 26 }) =
+  let pow26: pos = pow2 26 in
+  assert_norm (pow2 32 == 64 * pow26);
+  assert_norm (pow2 64 == 4096 * pow26 * pow26);
+  pow26
+
 inline_for_extraction
 let max26 = pow26 - 1
-
-assume val lemma_pow_32_26: _:unit{pow2 32 == 64 * pow26}
-assume val lemma_pow_64_26: _:unit{pow2 64 == 4096 * pow26 * pow26}
 
 
 let tup64_5 = (uint64 & uint64 & uint64 & uint64 & uint64)
@@ -103,10 +106,10 @@ inline_for_extraction
 let felem_wide5 (w:lanes) = felem5 w
 
 let felem_fits1 (#w:lanes) (x:uint64xN w) (m:scale32) =
-  forall (i:nat). i < w ==> uint_v (vec_v x).[i] <= m * max26
+  forall (i:nat). {:pattern (vec_v x).[i] } i < w ==> uint_v (vec_v x).[i] <= m * max26
 
 let felem_wide_fits1 (#w:lanes) (x:uint64xN w) (m:scale64) =
-  forall (i:nat). i < w ==> uint_v (vec_v x).[i] <= m * max26 * max26
+  forall (i:nat). {:pattern (vec_v x).[i] } i < w ==> uint_v (vec_v x).[i] <= m * max26 * max26
 
 let felem_fits5 (#w:lanes) (f:felem5 w) (m:scale32_5) =
   let (x1,x2,x3,x4,x5) = f in
